Squash everything -1
forall_variable_substitution

Knaster_tarski

pile_* lemmas

Svar_subst

Pre_fixp

mu_monotone

prf_equiv_of_impl_of_equiv

minor

freshness: seq

fix

WIP freshness refactoring

fix

WIP

WIP

WIP ltac congruence lemma

not_generic_in_prop

WIP, sets back

proof parameters

go back to sets

evar_fresh_seq_max

use

medoeip_evar_open

comment

medoeip_S_in

progress

finish the ex case

generalization: preparation for mu

mu template

WIP

svar_fresh_seq_max

medosip_svar_open

WIP

mmdoeip_S_in

mu: use IH

free_svars_free_evar_subst

WIP

WIP almost mu

finish all cases of the congruence lemma

prf_equiv_congruence

remove old code

ex_quan_monotone

convert many lemmas

WIP

MyGoal_rewriteIff

mgRewrite works again; wip simplify pile side condition

rewriting is slow but works

some lemmas

more lemmas

forall_gen

WIP pile_evs_svs_kt_back

pile_evs_svs_kt_back

useGenericReasoning

forall_variable_substitution'

forall_elim

prenex_forall_imp

Ex_gen_lifted

finish ProofMode.v

WIP definedness

hypothesis

remove a message

defined_evar

WIP lemmas

Singleton_ctx

Existence

in_context_impl_defined

total_phi_impl_phi_meta

begin working on deduction thm

WIP deduction thm

WIP and comment

framing_patterns

mgUseGenericReasoning

fix the MP case

have framing_left

Framing_right

svar_subst

finish Deduction theorem

membership_introduction

membership_elimination

membership_not_1

membership_not_2

membership_not_iff

membership_or_iff

membership_and_1

membership_and_iff

evar_fresh_seq_disj

fix

WIP

WIP

some comments

abstract stuff

move framing_patterns

abstract (set_solver)

abstract (wf_auto2).

more abstract

more abstract

more abstract

more abstract

abstract in specialize - rather feed?

remember i'; more abstract

matching-logic/src/ProofSystem.v
@@ -134,6 +134,31 @@ Section ml_proof_system.
 Lemma cast_proof {Γ} {ϕ} {ψ} (e : ψ = ϕ) : ML_proof_system Γ ϕ -> ML_proof_system Γ ψ.
 Proof. intros H. rewrite <- e in H. exact H. Defined.
 
+Fixpoint framing_patterns Γ ϕ (pf : Γ ⊢ ϕ) : list Pattern :=
+  match pf with
+  | hypothesis _ _ _ _ => []
+  | P1 _ _ _ _ _ => []
+  | P2 _ _ _ _ _ _ _ => []
+  | P3 _ _ _ => []
+  | Modus_ponens _ _ _ m0 m1
+    => (@framing_patterns _ _ m0) ++ (@framing_patterns _ _ m1)
+  | Ex_quan _ _ _ _ => []
+  | Ex_gen _ _ _ x _ _ pf _ => @framing_patterns _ _ pf
+  | Prop_bott_left _ _ _ => []
+  | Prop_bott_right _ _ _ => []
+  | Prop_disj_left _ _ _ _ _ _ _ => []
+  | Prop_disj_right _ _ _ _ _ _ _ => []
+  | Prop_ex_left _ _ _ _ _ => []
+  | Prop_ex_right _ _ _ _ _ => []
+  | Framing_left _ _ _ psi _ m0 => psi :: (@framing_patterns _ _ m0)
+  | Framing_right _ _ _ psi _ m0 => psi :: (@framing_patterns _ _ m0)
+  | Svar_subst _ _ _ _ _ _ m0 => @framing_patterns _ _ m0
+  | Pre_fixp _ _ _ => []
+  | Knaster_tarski _ _ phi psi m0 => @framing_patterns _ _ m0
+  | Existence _ => []
+  | Singleton_ctx _ _ _ _ _ _ => []
+  end.
+
 
   Fixpoint uses_ex_gen (EvS : EVarSet) Γ ϕ (pf : ML_proof_system Γ ϕ) :=
     match pf with
